pulse/lib/pulse/lib/Pulse.Lib.Reference.Array.fsti
@@ -1,0 +1,40 @@
+(*
+   Copyright 2023 Microsoft Research
+
+   Licensed under the Apache License, Version 2.0 (the "License");
+   you may not use this file except in compliance with the License.
+   You may obtain a copy of the License at
+
+       http://www.apache.org/licenses/LICENSE-2.0
+
+   Unless required by applicable law or agreed to in writing, software
+   distributed under the License is distributed on an "AS IS" BASIS,
+   WITHOUT WARRANTIES OR CONDITIONS OF ANY KIND, either express or implied.
+   See the License for the specific language governing permissions and
+   limitations under the License.
+*)
+
+module Pulse.Lib.Reference.Array
+#lang-pulse
+open FStar.Ghost
+open Pulse.Lib.Array.Basic
+open Pulse.Class.PtsTo
+open Pulse.Lib.Core
+open Pulse.Lib.Reference
+
+inline_for_extraction
+unobservable
+fn to_array u#a (#a: Type u#a) (r: ref a) #p (#v: erased a)
+  requires r |-> Frac p v
+  returns arr: array a
+  ensures rewrites_to arr (to_array_ghost r)
+  ensures arr |-> Frac p (seq![reveal v])
+  ensures pure (length arr == 1)
+
+inline_for_extraction
+ghost
+fn return_to_array u#a (#a: Type u#a) (r: ref a) #p (#v: Seq.seq a)
+  requires to_array_ghost r |-> Frac p v
+  requires pure (length (to_array_ghost r) == 1)
+  returns _: squash (Seq.length v == 1)
+  ensures r |-> Frac p (Seq.index v 0)
