pulse/test/ExtractUninit.fst
@@ -1,0 +1,30 @@
+module ExtractUninit
+open Pulse
+#lang-pulse
+
+fn uninit_ref ()
+  returns i: UInt32.t
+  ensures pure (i == 32ul)
+{
+  let r = Pulse.Lib.Reference.alloc_uninit UInt32.t ();
+  r := 3ul;
+  let res = (!r) `UInt32.add` 29ul;
+  Pulse.Lib.Reference.free r;
+  res
+}
+
+fn uninit_array ()
+  returns i: UInt32.t
+  ensures pure (i == 6ul)
+{
+  let arr = mask_alloc UInt32.t 5sz;
+  mask_write arr 0sz 1ul;
+  mask_write arr 1sz 2ul;
+  mask_write arr 2sz 3ul;
+  mask_write arr 3sz 4ul;
+  mask_write arr 4sz 5ul;
+  from_mask arr;
+  let result = arr.(1sz) `UInt32.add` arr.(3sz);
+  Pulse.Lib.Array.free arr;
+  result
+}
